Lots more Actions, partial refactoring for “history”

src/Actions/Actions.dfy
@@ -11,15 +11,22 @@ module Actions {
   import opened Seq
   import opened Math
 
+
+  // TODO: NOT a fully general-purpose handle on any arbitrary Dafny method,
+  // because gaps in Dafny expressiveness make that impossible for now
+  // (e.g. field references in framing clauses aren't expressions,
+  // decreases metrics aren't directly expressible in user code)
+  // Consider naming this something more specific, related to the assumptions:
+  //  1. Validatable (and doesn't modify anything not in Repr)
+  //  2. Behavior specified only by referring to consumed and produced.
   trait {:termination false} Action<T, R> extends Validatable {
 
-    ghost var consumed: seq<T>
-    ghost var produced: seq<R>
+    ghost var history: seq<(T, R)>
 
     ghost predicate Valid() 
       reads this, Repr 
       ensures Valid() ==> this in Repr 
-      ensures Valid() ==> CanProduce(consumed, produced)
+      ensures Valid() ==> CanProduce(history)
       decreases height, 0
 
     // KEY DESIGN POINT: these predicates specifically avoid reading the current
@@ -33,40 +40,53 @@ module Actions {
     // The downside is that these are then forced to use quantifiers
     // to talk about all possible states of an action.
 
-    ghost predicate CanConsume(consumed: seq<T>, produced: seq<R>, next: T)
-      requires |consumed| == |produced|
-      requires CanProduce(consumed, produced)
+    // TODO: Necessary but not sufficient that:
+    // CanConsume(history, nextIn) ==> exists nextOut :: CanProduce(history + [(nextIn, nextOut)])
+    // Does that need to be explicitly part of the spec?
+    ghost predicate CanConsume(history: seq<(T, R)>, next: T)
+      requires CanProduce(history)
       decreases height
 
-    ghost predicate CanProduce(consumed: seq<T>, produced: seq<R>)
-      ensures CanProduce(consumed, produced) ==> |consumed| == |produced|
+    ghost predicate CanProduce(history: seq<(T, R)>)
       decreases height
 
     ghost method Update(t: T, r: R) 
-      modifies `consumed, `produced
-      ensures consumed == old(consumed) + [t]
-      ensures produced == old(produced) + [r]
+      modifies `history
+      ensures history == old(history) + [(t, r)]
     {
-      consumed := consumed + [t];
-      produced := produced + [r];
+      history := history + [(t, r)];
     }
 
     method Invoke(t: T) returns (r: R) 
       requires Valid()
-      requires CanConsume(consumed, produced, t)
+      requires CanConsume(history, t)
       modifies Repr
       decreases height
       ensures Valid()
       ensures fresh(Repr - old(Repr))
-      ensures consumed == old(consumed) + [t]
-      ensures produced == old(produced) + [r]
+      ensures history == old(history) + [(t, r)]
   }
 
   // Common action invariants
 
-  ghost predicate OnlyProduces<T(!new), R(!new)>(i: Action<T, R>, c: R) {
-    forall consumed: seq<T>, produced: seq<R> | |consumed| == |produced| :: 
-      i.CanProduce(consumed, produced) <==> forall x <- produced :: x == c
+  function Consumed<T, R>(history: seq<(T, R)>): seq<T> {
+    Seq.Map((e: (T, R)) => e.0, history)
+  }
+
+  function Produced<T, R>(history: seq<(T, R)>): seq<R> {
+    Seq.Map((e: (T, R)) => e.1, history)
+  }
+
+  ghost predicate OnlyProduces<T, R>(i: Action<T, R>, history: seq<(T, R)>, c: R) 
+  {
+    i.CanProduce(history) <==> forall e <- history :: e.1 == c
+  }
+
+  ghost predicate CanConsumeAll<T(!new), R(!new)>(a: Action<T, R>, input: seq<T>) {
+    forall i | 0 < i < |input| ::
+      var consumed := input[..(i - 1)];
+      var next := input[i];
+      forall history | a.CanProduce(history) && Consumed(history) == consumed :: a.CanConsume(history, next)
   }
 
   ghost predicate Terminated<T>(s: seq<T>, c: T, n: nat) {
@@ -82,15 +102,16 @@ module Actions {
     assert forall i | 0 <= i < |right| :: right[i] == (left + right)[i + |left|];
   }
 
+  // TODO: generalize to "EventuallyProducesSequence"?
   ghost predicate ProducesTerminatedBy<T(!new), R(!new)>(i: Action<T, R>, c: R, limit: nat) {
-    forall consumed: seq<T>, produced: seq<R> | |consumed| == |produced| ::
-      i.CanProduce(consumed, produced) ==> exists n: nat | n <= limit :: Terminated(produced, c, n)
+    forall history: seq<(T, R)> | i.CanProduce(history) 
+      :: exists n: nat | n <= limit :: Terminated(Produced(history), c, n)
   }
 
   // Class of actions whose precondition doesn't depend on history (probably needs a better name)
   ghost predicate ContextFree<T(!new), R(!new)>(a: Action<T, R>, p: T -> bool) {
-    forall consumed, produced, next | a.CanProduce(consumed, produced)
-      :: a.CanConsume(consumed, produced, next) <==> p(next)
+    forall history, next | a.CanProduce(history)
+      :: a.CanConsume(history, next) <==> p(next)
   }
 
   // Aggregators
@@ -108,41 +129,37 @@ module Actions {
       reads this, Repr 
       ensures Valid() ==> this in Repr 
       ensures Valid() ==> 
-        && |consumed| == |produced|
-        && CanProduce(consumed, produced)
+        && CanProduce(history)
       decreases height, 0
     {
       && this in Repr
       && storage in Repr
       && 0 < storage.Length
       && 0 <= index <= storage.Length
-      && consumed == storage[..index]
-      && produced == Seq.Repeat((), |consumed|)
+      && Consumed(history) == storage[..index]
     }
 
     constructor() 
       ensures Valid()
       ensures fresh(Repr - {this})
-      ensures produced == []
+      ensures history == []
     {
       index := 0;
       storage := new T[10];
 
-      consumed := [];
-      produced := [];
+      history := [];
       Repr := {this, storage};
     }
 
-    ghost predicate CanConsume(consumed: seq<T>, produced: seq<()>, next: T)
+    ghost predicate CanConsume(history: seq<(T, ())>, next: T)
       decreases height
     {
       true
     }
-    ghost predicate CanProduce(consumed: seq<T>, produced: seq<()>)
-      ensures CanProduce(consumed, produced) ==> |consumed| == |produced|
+    ghost predicate CanProduce(history: seq<(T, ())>)
       decreases height
     {
-      produced == Seq.Repeat((), |consumed|)
+      true
     }
 
     twostate predicate ValidReprChange(before: set<object>, after: set<object>) {
@@ -151,14 +168,13 @@ module Actions {
 
     method Invoke(t: T) returns (r: ()) 
       requires Valid()
-      requires CanConsume(consumed, produced, t)
+      requires CanConsume(history, t)
       modifies Repr
       decreases height
       ensures Valid()
       ensures fresh(Repr - old(Repr))
-      ensures consumed == old(consumed) + [t]
-      ensures produced == old(produced) + [r]
-      ensures CanProduce(consumed, produced)
+      ensures history == old(history) + [(t, r)]
+      ensures CanProduce(history)
     {
       if index == storage.Length {
         var newStorage := new T[storage.Length * 2];
@@ -179,7 +195,7 @@ module Actions {
     function Values(): seq<T>
       requires Valid()
       reads Repr
-      ensures Values() == consumed
+      ensures Values() == Consumed(history)
     {
       storage[..index]
     }
@@ -194,4 +210,16 @@ module Actions {
     var _ := a.Invoke(5);
     assert a.Values() == [1, 2, 3, 4, 5];
   }
+
+  // Other primitives/examples todo:
+  //  * Eliminate all the (!new) restrictions - look into "older" parameters?
+  //    * How to state the invariant that a constructor as an action creates a new object every time?
+  //      * Lemma that takes produced as input, instead of forall produced?
+  //  * Enumerable ==> defines e.Enumerator()
+  //    * BUT can have infinite containers, probably need IEnumerable as well? (different T for the Action)
+  //  * Expressing that an Action "Eventually produces something" (look at how VMC models this for randomness)
+  //    * IsEnumerator(a) == "a eventually produces None" && "a then only produces None"
+  //    * Build on that to make CrossProduct(enumerable1, enumerable2)
+  //  * Example of adapting an iterator
+
 }
