src/Actions/Combinators.dfy
@@ -1,0 +1,51 @@
+include "Actions.dfy"
+include "Enumerators.dfy"
+
+module ActionCombinators {
+
+  import opened Actions
+  import opened Wrappers
+  import opened Enumerators
+
+  // a.produced == Seq.Map(f, a.consumed)
+  method Function<T, R>(f: T --> R)
+    returns (a: Action<T, R>)
+    ensures fresh(a.Repr)
+
+  method EnumeratorOfSeq(s: seq<T>)
+    returns (e: Enumerator<T>)
+
+  // a.k.a. Chain(first, second)
+  //
+  // To map a function f over the values of an action a: 
+  //   Compose(Function(f), a)
+  //
+  // Or over an enumerator e:
+  //   var maybeF := (maybeT: Option<T>) => match maybeT {
+  //      case Some(t) => Some(f(t))
+  //      case None => None
+  //   };
+  //   Compose(Function(maybeF), e)
+  //
+  // To map an Action a over a sequence s:
+  //   Collect(Compose(a, EnumeratorOfSeq(s)))
+  method Compose<T, V, R>(second: Action<V, R>, first: Action<T, V>)
+    returns (composed: Action<T, R>)
+    requires second.Repr !! first.Repr
+
+  // Produces Seq.Filter(what a produces, p)
+  // a has to be an Enumerator to ensure Invoke() eventually terminates
+  method Filter<T>(e: Enumerator<T>, p: T -> bool)
+    returns (filtered: Enumerator<T>)
+
+  // Produces Seq.Flatten(Actions.Map(inner, (what outer produces)))
+  // inner needs to be an action rather than just a function
+  // since enumerators are usually objects that need allocation.
+  method Nested<T, V>(outer: Enumerator<V>, inner: Action<V, Enumerator<T>>)
+    returns (nested: Enumerator<T>)
+
+  method ForEach(source: Enumerator<T>, sink: Aggregator<T>)
+
+  method Collect(source: Enumerator<T>)
+    returns (s: seq<T>)
+}
