src/Actions/DecreasesClauses.dfy
@@ -1,0 +1,58 @@
+
+module Termination {
+
+  datatype ClauseTail = More(next: TerminationMetric) | Top
+
+  datatype TerminationMetric = TerminationMetric(first: TMValue, rest: ClauseTail) {
+    predicate IsSmallerThan(other: TerminationMetric) {
+      if first == other.first then
+        match (rest, other.rest) {
+          case (Top, _) => false
+          case (More(_), Top) => true
+          case (More(next), More(otherNext)) => next.IsSmallerThan(otherNext)
+        }
+      else
+        first.IsSmallerThan(other.first)
+    }
+
+    ghost function {:axiom} Ordinal(): ORDINAL
+  }
+
+  lemma {:axiom} OrdinalOrdered(left: TerminationMetric, right: TerminationMetric) 
+    requires left.IsSmallerThan(right)
+    ensures left.Ordinal() < right.Ordinal()
+
+  datatype TMValue = 
+    | TMNat(natValue: nat)
+    | TMChar(charValue: nat)
+    | TMSeq(seqValue: seq<TMValue>) 
+    // TODO: etc
+  {
+    predicate IsSmallerThan(other: TMValue) {
+      match (this, other) {
+        case (TMNat(left), TMNat(right)) => left < right
+        case (TMChar(left), TMChar(right)) => left < right
+        case (TMSeq(left), TMSeq(right)) => left < right // TODO: should be Seq.IsSubsequenceOf
+        // TODO: etc
+        case _ => false
+      }
+    }
+  }
+}
+
+module Example {
+
+  datatype D = Less(x: nat) | More(x: nat)
+
+  function Foo(d: D): nat 
+    decreases d
+  {
+    if d.More? then
+      Foo(Less(d.x))
+    else
+      if d.x == 0 then  
+        42
+      else
+        Foo(Less(d.x - 1))
+  }
+}
