src/Actions/GenericAction.dfy
@@ -1,0 +1,31 @@
+
+include "../Wrappers.dfy"
+include "../Frames.dfy"
+include "../Math.dfy"
+include "../Collections/Sequences/Seq.dfy"
+
+include "DecreasesClauses.dfy"
+
+module GenericActions {
+
+  import opened Wrappers
+  import opened Frames
+  import opened Seq
+  import opened Math
+  import opened Termination
+
+  trait {:termination false} Action<T, R> extends Validatable {
+
+    ghost predicate Requires(t: T)
+    ghost function Reads(t: T): set<object>
+    ghost function Modifies(t: T): set<object>
+    ghost function Decreases(t: T): TerminationMetric
+    ghost predicate Ensures(t: T, r: R)
+
+    method Invoke(t: T) returns (r: R) 
+      requires Requires(t)
+      modifies Modifies(t)
+      decreases Decreases(t).Ordinal()
+  }
+
+}
