src/Actions/ObjectQuantification.dfy
@@ -1,0 +1,9 @@
+module Testing {
+
+  trait SimpleAction<T> {
+    method Invoke() returns (t: T)
+  }
+
+  method 
+
+}
